Binary heap has no admits.  Requires ~1m30s to build.
Still missing: heapify, peek, make, free, increase/decrease key, lookup, merge?

sample_mark/verif_binary_heap.v
@@ -1,327 +1,11 @@
+Require Import RelationClasses.
 Require Import VST.floyd.proofauto.
 Require Import RamifyCoq.sample_mark.binary_heap_model.
+Require Import RamifyCoq.sample_mark.binary_heap_Zmodel.
 Require Import RamifyCoq.sample_mark.binary_heap.
-Require Import RelationClasses.
-(* Require Import VST.floyd.sublist. *)
+Require Import RamifyCoq.sample_mark.env_binary_heap.
 
 Set Nested Proofs Allowed.
-
-(* Versions in Z... *)
-
-Definition Zexchange {A : Type} (L : list A) (i j : Z) : list A :=
-  exchange L (Z.to_nat i) (Z.to_nat j).
-
-Lemma Zlength_Zexchange {A : Type} : forall (L : list A) i j,
-  Zlength (Zexchange L i j) = Zlength L.
-Proof.
-  intros. unfold Zexchange. do 2 rewrite Zlength_correct. rewrite exchange_length. trivial.
-Qed.
-
-Lemma Zlength_one: forall A (a : A),
-  Zlength [a] = 1.
-Proof. reflexivity. Qed.
-
-Lemma Znth_nth_error {A} `{Ia : Inhabitant A} : forall (L : list A) (i : Z),
-  0 <= i < Zlength L ->
-  nth_error L (Z.to_nat i) = Some (Znth i L).
-Proof.
-  intros. rewrite <- nth_Znth; trivial.
-  apply nth_error_nth.
-  rewrite <- ZtoNat_Zlength. lia.
-Qed.
-
-Lemma nth_error_Znth {A} `{Ia : Inhabitant A}: forall (L1 L2 : list A) i j,
-  0 <= i < Zlength L1 ->
-  0 <= j < Zlength L2 ->
-  nth_error L1 (Z.to_nat i) = nth_error L2 (Z.to_nat j) <->
-  Znth i L1 = Znth j L2.
-Proof.
-  intros.
-  assert (Z.to_nat i < length L1 /\ Z.to_nat j < length L2)%nat. {
-    generalize (Zlength_length _ L1 (Zlength L1)); intro.
-    generalize (Zlength_length _ L2 (Zlength L2)); intro.
-    destruct H1. apply Zlength_nonneg.
-    destruct H2. apply Zlength_nonneg.
-    rewrite (H1 eq_refl). rewrite (H2 eq_refl). lia. }
-  repeat rewrite <- nth_Znth; trivial.
-  generalize (nth_error_nth A Ia); intros.
-  split; intros. do 2 (rewrite H2 in H3; try lia). inversion H3. congruence.
-  rewrite H2. rewrite H2. congruence. lia. lia.
-Qed.
-
-Lemma Znth_Zexchange : forall {A} `{Ia : Inhabitant A} (L : list A) i j,
-  0 <= i < Zlength L ->
-  0 <= j < Zlength L ->
-  Znth i (Zexchange L i j) = Znth j L.
-Proof.
-  intros.
-  apply nth_error_Znth; auto. rewrite Zlength_Zexchange. trivial.
-  generalize (Zlength_length _ L (Zlength L)). intro.
-  apply nth_error_exchange; lia.
-Qed.
-
-Lemma Znth_Zexchange' : forall {A} `{Ia : Inhabitant A} (L : list A) i j,
-  0 <= i < Zlength L ->
-  0 <= j < Zlength L ->
-  Znth j (Zexchange L i j) = Znth i L.
-Proof.
-  intros.
-  apply nth_error_Znth; auto. rewrite Zlength_Zexchange. trivial.
-  generalize (Zlength_length _ L (Zlength L)). intro.
-  apply nth_error_exchange'; lia.
-Qed.
-
-Lemma Znth_Zexchange'' : forall {A} `{Ia : Inhabitant A} (L : list A) k i j,
-  0 <= i < Zlength L ->
-  0 <= j < Zlength L ->
-  k <> i -> k <> j ->
-  Znth k (Zexchange L i j) = Znth k L.
-Proof.
-  intros.
-  assert (k < 0 \/ 0 <= k < Zlength L \/ Zlength L <= k) by lia.
-  destruct H3 as [? | [? | ?]].
-  repeat rewrite Znth_underflow; trivial.
-  2: repeat rewrite Znth_overflow; try rewrite Zlength_Zexchange; trivial; lia.
-  apply nth_error_Znth; auto. rewrite Zlength_Zexchange. trivial.
-  apply nth_error_exchange''.
-  intro. apply H1. apply Z2Nat.inj; lia.
-  intro. apply H2. apply Z2Nat.inj; lia.
-Qed.
-
-Lemma Zexchange_eq: forall A (L : list A) i,
-  Zexchange L i i = L.
-Proof. unfold Zexchange. intros. apply exchange_eq. Qed.
-
-Lemma upd_Znth_overwrite:
-  forall {A} (l : list A) i a b,
-    0 <= i < Zlength l ->
-    upd_Znth i (upd_Znth i l a) b = upd_Znth i l b.
-Proof.
-  intros.
-  rewrite upd_Znth_unfold by now rewrite upd_Znth_Zlength.
-  rewrite upd_Znth_Zlength; trivial.
-  repeat rewrite upd_Znth_unfold by trivial.
-  rewrite sublist0_app1.
-  2: rewrite Zlength_sublist; lia.
-  rewrite sublist_sublist00 by lia.
-  f_equal. f_equal.
-  rewrite app_assoc.
-  rewrite sublist_app2.
-  2: { rewrite Zlength_app, Zlength_sublist by lia.
-       unfold Zlength. simpl. lia.
-  }
-  rewrite Zlength_app, Zlength_sublist by lia.
-  unfold Zlength at 1; simpl.
-  rewrite sublist_same; trivial.
-  - lia.
-  - unfold Zlength at 2; simpl.
-    rewrite Zlength_sublist by lia. lia.
-Qed.
-
-Lemma upd_Znth_same_Znth:
-  forall {A} `{Ia : Inhabitant A} (l: list A) i,
-    0 <= i < Zlength l ->
-    upd_Znth i l (Znth i l) = l.
-Proof.
-  intros. rewrite upd_Znth_unfold by trivial.
-  rewrite <- sublist_len_1 by trivial.
-  repeat rewrite <- sublist_split.
-  apply sublist_same; trivial.
-  all: lia.
-Qed.
-
-Lemma exchange_eq_nil: forall A (L : list A) i j,
-  exchange L i j = [] ->
-  L = [].
-Proof. unfold exchange. intros A L i j. case nth_error; auto. case nth_error; auto.
-  destruct L. trivial. destruct j, i; simpl; discriminate.
-Qed.
-
-Lemma nth_error_eq: forall A (L1 L2 : list A),
-  (forall i, nth_error L1 i = nth_error L2 i) ->
-  L1 = L2.
-Proof.
-  induction L1. destruct L2; auto; intros. specialize (H 0%nat); discriminate.
-  destruct L2. intro. specialize (H 0%nat); discriminate. intros.
-  f_equal. specialize (H 0%nat). inversion H. trivial.
-  apply IHL1. intro. specialize (H (S i)). apply H.
-Qed.
-
-Lemma Zexchange_head_foot: forall A (head : A) body foot,
-  Zexchange ((head :: body) ++ [foot]) 0 (Zlength (head :: body)) = ((foot :: body) ++ [head]).
-Proof.
-  intros.
-  apply nth_error_eq. intro i'. unfold Zexchange. simpl Z.to_nat. case (eq_nat_dec i' 0); intro.
-  + subst i'. 
-    rewrite nth_error_exchange; simpl. 2: lia.
-    rewrite app_comm_cons. rewrite ZtoNat_Zlength.
-    rewrite nth_error_app2. simpl. rewrite Nat.sub_diag. trivial. lia.
-    rewrite ZtoNat_Zlength. rewrite app_length. simpl. lia.
-  + case (eq_nat_dec i' (Z.to_nat (Zlength (head :: body)))); intro.
-    - subst i'.
-      rewrite nth_error_exchange'; simpl. 2: lia.
-      rewrite app_comm_cons. rewrite ZtoNat_Zlength.
-      rewrite nth_error_app2. simpl. rewrite Nat.sub_diag. trivial. simpl. lia.
-      rewrite ZtoNat_Zlength. rewrite app_length. simpl. lia.
-    - rewrite nth_error_exchange''; auto.
-      destruct i'. contradiction. simpl. rewrite ZtoNat_Zlength in n0. simpl in n0.
-      assert (i' < (length body) \/ i' >= length (body ++ [foot]))%nat. { rewrite app_length. simpl. lia. }
-      destruct H. repeat rewrite nth_error_app1; auto.
-      assert (i' >= length (body ++ [head]))%nat. { rewrite app_length in *. simpl in *. lia. }
-      apply nth_error_None in H. apply nth_error_None in H0. congruence.
-Qed.
-
-Lemma Permutation_Zlength: forall A (L1 : list A) L2,
-  Permutation L1 L2 ->
-  Zlength L1 = Zlength L2.
-Proof.
-  intros. apply Permutation_length in H. do 2 rewrite Zlength_correct. congruence.
-Qed.
-
-
-(* Relation on heap items. *)
-Definition heap_item : Type := (int * int)%type.
-Definition cmp (a b : heap_item) : bool :=
-  negb (Int.lt (fst b) (fst a)).
-Definition cmp_rel (a b : heap_item) : Prop :=
-  cmp a b = true.
-Lemma cmp_dec: forall a a', {cmp_rel a a'} + {~cmp_rel a a'}.
-Proof.
-  intros [? ?] [? ?]. unfold cmp_rel, cmp. simpl. case (Int.lt i1 i); simpl; auto.
-Qed. 
-Instance cmp_po: PreOrder cmp_rel.
-Proof.
-  constructor. intros [? ?]. red. unfold cmp. simpl. case_eq (Int.lt i i); auto; intro. exfalso.
-  apply lt_inv in H. lia.
-  intros [? ?] [? ?] [? ?]. unfold cmp_rel, cmp. simpl. 
-  case_eq (Int.lt i3 i); auto.
-  case_eq (Int.lt i1 i); auto.
-  case_eq (Int.lt i3 i1); auto. simpl.
-  intros ? ? ?. exfalso.
-  apply lt_inv in H1.
-  apply lt_false_inv in H.
-  apply lt_false_inv in H0.
-  lia.
-Qed.
-Lemma cmp_linear: forall a b,
-  cmp_rel a b \/ cmp_rel b a.
-Proof.
-  intros [? ?] [? ?]. unfold cmp_rel, cmp; simpl.
-  case_eq (Int.lt i1 i); auto. intro. 
-  right.
-  case_eq (Int.lt i i1); auto. intro. exfalso. 
-  apply lt_inv in H. apply lt_inv in H0.
-  lia.
-Qed.
-
-(* Not sure if it's a great idea to expose the capacity inside the abstraction boundary. *)
-Definition heap : Type := (nat * list heap_item)%type.
-Instance heap_inhabitant : Inhabitant heap := (O, []).
-Definition heap_capacity (h : heap) : Z := Z.of_nat (fst h).
-Definition heap_items (h : heap) : list heap_item := snd h.
-Definition heap_size (h : heap) : Z := Zlength (heap_items h).
-
-(*
-Definition heap_permutation (h1 h2 : heap) : Prop :=
-  heap_capacity h1 = heap_capacity h2 /\ Permutation (heap_items h1) (heap_items h2).
-*)
-
-Definition heap_ordered := binary_heap_model.heapOrdered heap_item cmp_rel.
-Definition weak_heap_ordered_bottom_up (L : list heap_item) (x : Z) := 
-  binary_heap_model.weak_heapOrdered2 heap_item cmp_rel L (Z.to_nat x).
-Definition weak_heap_ordered_top_down (L : list heap_item) (x : Z) := 
-  binary_heap_model.weak_heapOrdered heap_item cmp_rel L (Z.to_nat x).
-Definition swim := binary_heap_model.swim heap_item cmp_rel cmp_dec.
-Definition sink L i := binary_heap_model.sink heap_item cmp_rel cmp_dec (L,i).
-(* Definition insert := binary_heap_model.insert heap_item cmp_rel cmp_dec. *)
-(* Definition remove_min := binary_heap_model.remove_min heap_item cmp_rel cmp_dec. *)
-Definition Zleft_child i  := Z.of_nat (binary_heap_model.left_child  (Z.to_nat i)).
-Lemma Zleft_child_unfold: forall i,
-  0 <= i ->
-  Zleft_child i = (2 * i) + 1.
-Proof.
-  unfold Zleft_child, binary_heap_model.left_child. intros.
-  do 2 rewrite Nat2Z.inj_add. rewrite Z2Nat.id; lia.
-Qed.
-Definition Zright_child i := Z.of_nat (binary_heap_model.right_child (Z.to_nat i)).
-Lemma Zright_child_unfold: forall i,
-  Zright_child i = Zleft_child i + 1.
-Proof.
-  unfold Zright_child, Zleft_child, binary_heap_model.right_child. intros.
-  rewrite Nat2Z.inj_add. trivial.
-Qed.
-Definition Zparent (i : Z) : Z := Z.of_nat (parent (Z.to_nat i)).
-Lemma Zparent_unfold: forall i,
-  0 < i ->
-  Zparent i = (i - 1) / 2.
-Proof.
-  unfold Zparent, parent. intros.
-  rewrite Nat.div2_div, div_Zdiv; auto.
-  rewrite Nat2Z.inj_sub. rewrite Z2Nat.id; lia.
-  lia.
-Qed.
-Lemma Zparent_0:
-  Zparent 0 = 0.
-Proof. reflexivity. Qed.
-Lemma Zparent_repr: forall i,
-  0 < i <= Int.max_unsigned ->
-  Int.repr (Zparent i) = Int.divu (Int.repr (i - 1)) (Int.repr 2).
-Proof.
-  intros. unfold Int.divu. repeat rewrite Int.unsigned_repr.
-  2,3: rep_lia. rewrite Zparent_unfold. trivial. lia.
-Qed.
-
-(* This may get bundled elsewhere at some point. *)
-Instance CompSpecs : compspecs. Proof. make_compspecs prog. Defined.
-Definition Vprog : varspecs. mk_varspecs prog. Defined.
-Global Existing Instance CompSpecs.
-
-Definition t_item := Tstruct _structItem noattr.
-Definition t_pq := Tstruct _structPQ noattr.
-
-Definition heap_item_rep (i : heap_item) : reptype t_item :=
-  (Vint (fst i), Vint (snd i)).
-
-Definition hitem (i : heap_item) : val -> mpred :=
-  data_at Tsh t_item (heap_item_rep i).
-
-Definition harray (contents : list heap_item) : val -> mpred :=
-  data_at Tsh (tarray t_item (Zlength contents)) (map heap_item_rep contents).
-
-Lemma harray_emp: forall arr,
-  harray [] arr |-- emp.
-Proof.
-  unfold harray. intros. rewrite data_at_isptr. entailer. rewrite data_at_zero_array_eq; auto.
-Qed.
-
-Lemma fold_harray': forall L i arr,
-  i = Zlength L ->
-  data_at Tsh (tarray t_item i) (map heap_item_rep L) arr = harray L arr.
-Proof. intros. rewrite H. reflexivity. Qed.
-
-Lemma fold_harray: forall L arr,
-  data_at Tsh (tarray t_item (Zlength L)) (map heap_item_rep L) arr = harray L arr.
-Proof. reflexivity. Qed.
-
-Lemma harray_split: forall L1 L2 ptr,
-  harray (L1 ++ L2) ptr = 
-  ((harray L1 ptr) * 
-   (harray L2 (field_address0 (tarray t_item (Zlength (L1 ++ L2))) [ArraySubsc (Zlength L1)] ptr)))%logic.
-Proof.
-  intros. unfold harray.
-  rewrite map_app.
-  erewrite split2_data_at_Tarray_app.
-  2: rewrite Zlength_map; reflexivity. 2: rewrite Zlength_app, Zlength_map; lia.
-  rewrite Zlength_app.
-  replace (Zlength L1 + Zlength L2 - Zlength L1) with (Zlength L2) by lia.
-  trivial.
-Qed.
-
-Definition valid_pq (pq : val) (h: heap): mpred :=
-  EX arr : val, EX junk: list heap_item,
-    (!! heap_ordered (heap_items h)) && (!! (Zlength ((heap_items h) ++ junk) = heap_capacity h)) &&
-    (data_at Tsh t_pq (Vint (Int.repr (heap_capacity h)), (Vint (Int.repr (heap_size h)), arr)) pq *
-       harray ((heap_items h) ++ junk) arr).
 
 Definition exch_spec :=
   DECLARE _exch WITH i : Z, j : Z, arr: val, arr_contents: list heap_item
@@ -419,7 +103,8 @@ Definition sink_spec :=
   PRE [tuint, tptr t_item, tuint]
     PROP (0 <= i <= Zlength arr_contents; 
           first_available = Zlength arr_contents;
-          (2 * first_available) <= Int.max_unsigned; (* i = fa - 1 -> (2 * i + 1) = 2 * fa - 1, must be representable *)
+          (i = Zlength arr_contents -> (2 * i) <= Int.max_unsigned);
+          (i < Zlength arr_contents -> (2 * (first_available - 1) <= Int.max_unsigned)); (* i = fa - 1 -> (2 * i + 1) = 2 * fa - 1, must be representable *)
           weak_heap_ordered_top_down arr_contents i)
     PARAMS (Vint (Int.repr i); arr; Vint (Int.repr first_available))
     GLOBALS ()
@@ -441,12 +126,29 @@ Proof.
   assert (Hc : i = Zlength arr_contents \/ 0 <= i < Zlength arr_contents) by lia. destruct Hc as [Hc | Hc].
 * (* Special case: oob sink, used when removing the last element of the heap. *)
   forward_while ( PROP () LOCAL (temp _k (Vint (Int.repr i)); temp _first_available (Vint (Int.repr first_available))) SEP (harray arr_contents arr) ).
-  entailer!. entailer. exfalso. lia.
+  entailer!. entailer!. exfalso. lia.
+(* This is where the bound is needed.  For some reason I need a slightly different bound than I expect. *)
+(*
+rewrite H0 in *. subst i. remember (Zlength arr_contents). destruct H. clear H3 H0 first_available H2 POSTCONDITION MORE_COMMANDS Delta Delta_specs arr Heqz arr_contents.
+lia.
+*)
+(*
+(* 2 * fa - 1 *)
+H : 0 <= z
+H1 : 2 * z - 1 <= Int.max_unsigned
+HRE : Int.unsigned (Int.repr (2 * z + 1)) < z
+
+(* 2 * fa *)
+H : 0 <= z
+H1 : 2 * z <= Int.max_unsigned
+HRE : 2 * z + 1 < z
+*)
   forward.
   Exists arr_contents. entailer!.
-  eapply weak_heapOrdered_oob. 2: apply H2. rewrite Zlength_correct. lia.
+  eapply weak_heapOrdered_oob. 2: apply H3.
+  rewrite Zlength_correct, Nat2Z.id. apply le_refl.
 * (* Main line *)
-  unfold Swhile.
+  assert (Hx : i < Zlength arr_contents) by lia. specialize (H2 Hx). clear H1 Hx. rename H2 into H1. rename H3 into H2.
   forward_loop (EX i' : Z, EX arr_contents' : list heap_item, 
                  PROP (0 <= i' < Zlength arr_contents; 
                        sink arr_contents (Z.to_nat i) = sink arr_contents' (Z.to_nat i'))
@@ -482,7 +184,7 @@ Proof.
         { entailer!. simpl. repeat f_equal. rewrite Zright_child_unfold, Zleft_child_unfold; lia. }
         { rewrite Int.unsigned_repr in H7. rewrite Zright_child_unfold, Zleft_child_unfold in *; lia.
           (* Here is where we seem to need the precise bound on first_available? *)
-          rewrite Zleft_child_unfold; rep_lia. }
+          rewrite Zleft_child_unfold in *; rep_lia. }
       forward. Exists (cmp (Znth (Zright_child i') arr_contents') (Znth (Zleft_child i') arr_contents')).
       unfold cmp_rel. rewrite Zright_child_unfold, Zleft_child_unfold in *.
       rewrite Int.unsigned_repr in H7. 2,3,4,5: rep_lia.
@@ -556,8 +258,7 @@ Proof.
     + subst j'. destruct b.
       - rewrite H5 in H7. apply nth_error_None in H0. destruct H7. unfold Zright_child in H7. rewrite Zlength_correct in H7. lia.
       - split. unfold Zleft_child. lia. tauto.
-(* Time Qed. *)
-Admitted.
+Time Qed.
 
 Lemma body_swim: semax_body Vprog Gprog f_swim swim_spec.
 Proof.
@@ -626,25 +327,25 @@ Proof.
     3: rewrite <- Znth_nth_error. 3: rewrite Nat2Z.id; trivial.
     1,2,3: lia.
   * rewrite Zparent_repr. trivial. lia.
-Qed.
+Time Qed.
 
 Lemma body_insert_nc: semax_body Vprog Gprog f_insert_nc insert_nc_spec.
 Proof.
   start_function.
   unfold valid_pq.
   Intros arr junk.
-  destruct junk. { exfalso. unfold heap_size, heap_capacity in *. rewrite Zlength_app, Zlength_nil in H1. lia. }
+  destruct junk. { exfalso. unfold heap_size, heap_capacity in *. rewrite Zlength_app, Zlength_nil in H2. lia. }
   change (h0 :: junk) with ([h0] ++ junk) in *. rewrite app_assoc in *.
   rewrite harray_split. Intros.
   assert (0 <= heap_size h) by apply Zlength_nonneg.
-  forward. unfold harray. entailer.
+  forward. unfold harray. entailer!.
   forward. unfold hitem.
   forward.
   unfold harray at 1.
   forward. entailer!. rewrite Zlength_app, Zlength_one. unfold heap_size in *. lia.
   forward.
   forward.
-  forward. { (* C typing issue? *) entailer!. apply H9. discriminate. }
+  forward. { (* C typing issue? *) entailer!. apply H10. discriminate. }
   forward. entailer!. rewrite Zlength_app, Zlength_one. unfold heap_size in *. lia.
   forward.
   forward.
@@ -667,20 +368,20 @@ Proof.
   (* Prove postcondition *)
   Exists ((Z.to_nat (heap_capacity h))%nat, vret).
   unfold heap_capacity. rewrite Nat2Z.id. simpl fst.
-  unfold valid_pq. entailer. Exists arr.
-  apply andp_right. { apply prop_right. split; trivial. unfold heap_items in *. simpl.
-    transitivity (snd h ++ [iv]); trivial. change (iv :: snd h) with ([iv] ++ snd h).
-    apply Permutation_app_comm. }
-  Exists junk. entailer!. { rewrite Zlength_app. apply Permutation_Zlength in H4.
-    unfold heap_items. simpl. rewrite <- H4. unfold heap_capacity in *. simpl. rewrite <- H1.
-    autorewrite with sublist. lia. }
-  unfold heap_size, heap_capacity, heap_items. simpl fst. simpl snd.
-  generalize (Permutation_Zlength _ _ _ H4); intro. rewrite <- H9.
-  replace (Zlength (heap_items h ++ [iv])) with (Zlength (snd h) + 1). 2: rewrite Zlength_app; trivial.
-  cancel.
-  rewrite harray_split. cancel.
-  repeat rewrite Zlength_app. rewrite <- H9. rewrite Zlength_app. apply derives_refl.
-Qed.
+  unfold valid_pq. entailer!.
+  * transitivity (snd h ++ [iv]); trivial. change (iv :: heap_items h) with ([iv] ++ heap_items h).
+    apply Permutation_app_comm.
+  * Exists arr junk. entailer!.
+    + rewrite Zlength_app. apply Permutation_Zlength in H5.
+      unfold heap_items. simpl. rewrite <- H5. unfold heap_capacity in *. simpl. rewrite <- H2.
+      autorewrite with sublist. lia.
+    + unfold heap_size, heap_capacity, heap_items. simpl fst. simpl snd.
+      generalize (Permutation_Zlength _ _ _ H5); intro. rewrite <- H10.
+      replace (Zlength (heap_items h ++ [iv])) with (Zlength (snd h) + 1). 2: rewrite Zlength_app; trivial.
+      cancel.
+      rewrite harray_split. cancel.
+      repeat rewrite Zlength_app. rewrite <- H10. rewrite Zlength_app. apply derives_refl.
+Time Qed.
 
 Lemma body_remove_min_nc: semax_body Vprog Gprog f_remove_min_nc remove_min_nc_spec.
 Proof.
@@ -718,14 +419,14 @@ Proof.
     { entailer!. rewrite Zlength_Zexchange. lia. }
     { entailer!. rewrite Znth_map. 2: rewrite Zlength_Zexchange; lia.
       rewrite <- Hx. rewrite Znth_Zexchange'; try lia. rewrite Znth_0_cons.
-      apply Forall_map in H5.
-      rewrite Forall_Znth in H5. specialize (H5 (Zlength l)). do 2 rewrite Zlength_map in H5. rewrite Zlength_Zexchange in H5.
+      apply Forall_map in H6.
+      rewrite Forall_Znth in H6. specialize (H6 (Zlength l)). do 2 rewrite Zlength_map in H6. rewrite Zlength_Zexchange in H6.
       assert (Hq: 0 <= (Zlength l) < Zlength (root :: l)) by lia.
-      specialize (H5 Hq). rewrite Znth_map in H5. 2: rewrite Zlength_map, Zlength_Zexchange; lia.
-      rewrite Znth_map in H5. 2: rewrite Zlength_Zexchange; lia.
-      rewrite Znth_Zexchange' in H5; try lia.
+      specialize (H6 Hq). rewrite Znth_map in H6. 2: rewrite Zlength_map, Zlength_Zexchange; lia.
+      rewrite Znth_map in H6. 2: rewrite Zlength_Zexchange; lia.
+      rewrite Znth_Zexchange' in H6; try lia.
       (* Flailing around solves the goal... *)
-      apply H5. discriminate. }
+      apply H6. discriminate. }
   (* this change refolds the harray back up *)
   change (data_at _ _ _ arr) with (harray (Zexchange (root :: l) 0 (Zlength l)) arr).
   forward.
@@ -745,11 +446,11 @@ Proof.
     forward_call (0, arr, @nil heap_item, 0); rewrite Zlength_nil. 
       { unfold harray. rewrite data_at_isptr. entailer. (* Surely there's a less heavy hammer way to do this? *)
         rewrite data_at_zero_array_eq; auto. entailer!. }
-      { split; auto. split; auto. split. rep_lia.
+      { split; auto. split; auto. split. rep_lia. split. rep_lia.
         apply hOwhO. apply cmp_po. apply heapOrdered_empty. }
     (* Prove postcondition *)
     Intro vret. Exists (n, vret) root. entailer. (* Surely there's a less heavy hammer way to do this? *)
-    destruct H. apply Permutation_nil in H12. subst vret. clear H Hy.
+    destruct H. apply Permutation_nil in H13. subst vret. clear H Hy.
     sep_apply harray_emp. rewrite emp_sepcon.
     rewrite Zlength_Zexchange. rewrite Zexchange_eq.
     do 2 rewrite fold_harray. unfold valid_pq, hitem.
@@ -760,38 +461,41 @@ Proof.
   * (* main line: heap still has items in it *)
     destruct l0; inversion H. subst h0.
     deadvars!.
-    assert (Zlength (h :: l) = Zlength (root :: l0)). { rewrite H4, Zlength_app, Zlength_one, Zlength_cons. lia. }
-    rewrite H2, Zexchange_head_foot. rewrite harray_split.
+    assert (Zlength (h :: l) = Zlength (root :: l0)). { rewrite H5, Zlength_app, Zlength_one, Zlength_cons. lia. }
+    rewrite H3, Zexchange_head_foot. rewrite harray_split.
     forward_call (0, arr, (foot :: l0), Zlength (foot :: l0)). entailer!.
       { split. rewrite Zlength_cons. generalize (Zlength_nonneg l0). lia.
-        split; trivial. split. admit. (* Need some bound... *)
+        split; trivial. split. rep_lia.
+        (* Here is where we use the bound. *)
+        split. intros _. generalize (Zlength_nonneg junk); intro.
+        simpl in H2. repeat rewrite Zlength_cons in *. rewrite Zlength_app in H2. lia.
         apply weak_heapOrdered_root with root.
-        rewrite H4, app_comm_cons in H0.
-        apply heapOrdered_cutfoot in H0. trivial. }
+        rewrite H5, app_comm_cons in H1.
+        apply heapOrdered_cutfoot in H1. trivial. }
     (* Prove postcondition *)
     Intro vret. Exists (n, vret) root. simpl fst. unfold hitem, heap_item_rep, heap_size, heap_capacity. simpl fst. simpl snd. entailer!.
       { (* Pure part *)
-        split. constructor. rewrite H4. transitivity ([foot] ++ l0). apply Permutation_app_comm. destruct H3. auto.
-        generalize (root_minimal _ _ _ _ H0 root eq_refl); intro.
-        rewrite H4 in H9. apply Forall_inv_tail in H9.
-        eapply forall_permutation. apply H9. transitivity ([foot] ++ l0). apply Permutation_app_comm. simpl. tauto. }
+        split. constructor. rewrite H5. transitivity ([foot] ++ l0). apply Permutation_app_comm. destruct H4. auto.
+        generalize (root_minimal _ _ _ _ H1 root eq_refl); intro.
+        rewrite H5 in H10. apply Forall_inv_tail in H10.
+        eapply forall_permutation. apply H10. transitivity ([foot] ++ l0). apply Permutation_app_comm. simpl. tauto. }
     unfold valid_pq. Exists arr (root :: junk). unfold heap_size, heap_capacity. simpl.
-    destruct H3.
-    replace (Zlength vret) with (Zlength (root :: l0)). 2: { apply Permutation_Zlength in H9. trivial. }
+    destruct H4.
+    replace (Zlength vret) with (Zlength (root :: l0)). 2: { apply Permutation_Zlength in H10. trivial. }
     entailer!. { (* Pure part inside spatial part *)
-      rewrite <- H1. apply Permutation_Zlength in H9. autorewrite with sublist. rewrite <- H9.
-      autorewrite with sublist in *. lia. }
+      simpl fst in H2. rewrite <- H2. apply Permutation_Zlength in H10. autorewrite with sublist. rewrite <- H10.
+      simpl snd. autorewrite with sublist in *. lia. }
     (* Spatial part, this seems a bit uglier than necessary? *)
     change (root :: junk) with ([root] ++ junk). rewrite app_assoc. do 2 rewrite harray_split.
-    apply Permutation_Zlength in H9.
-    rewrite app_comm_cons. rewrite Zlength_app. rewrite H9. rewrite Zlength_app.
-    assert (Zlength (root :: l0) = Zlength vret). { rewrite <- H9. do 2 rewrite Zlength_cons. trivial. }
+    apply Permutation_Zlength in H10.
+    rewrite app_comm_cons. rewrite Zlength_app. rewrite H10. rewrite Zlength_app.
+    assert (Zlength (root :: l0) = Zlength vret). { rewrite <- H10. do 2 rewrite Zlength_cons. trivial. }
     do 3 rewrite app_comm_cons.
-    do 4 rewrite Zlength_app. rewrite H10.
+    do 4 rewrite Zlength_app. rewrite H11.
     do 2 rewrite Zlength_one.
     rewrite Zlength_cons.
-    rewrite H2, H10. cancel.
-Admitted.
+    rewrite H3, H11. cancel.
+Time Qed.
 
 Lemma body_less: semax_body Vprog Gprog f_less less_spec.
 Proof.
@@ -806,7 +510,7 @@ Proof.
   forward.
   repeat rewrite Znth_map in *; trivial.
   entailer!.
-Qed.
+Time Qed.
 
 Lemma body_size: semax_body Vprog Gprog f_size size_spec.
 Proof.
@@ -818,7 +522,7 @@ Proof.
   unfold valid_pq.
   Exists arr. Exists junk.
   entailer!.
-Qed.
+Time Qed.
 
 Lemma body_capacity: semax_body Vprog Gprog f_capacity capacity_spec.
 Proof.
@@ -830,7 +534,7 @@ Proof.
   unfold valid_pq.
   Exists arr. Exists junk.
   entailer!.
-Qed.
+Time Qed.
 
 (* I need this to make a replace work... ugly... *)
 Lemma heap_item_rep_morph: forall x y,
@@ -905,4 +609,4 @@ Proof.
       rewrite upd_Znth_diff. rewrite upd_Znth_same. rewrite Znth_Zexchange; trivial. 1,2,3,4: autorewrite with sublist; trivial.
       rewrite Znth_Zexchange''; auto.
       repeat rewrite upd_Znth_diff; autorewrite with sublist; trivial.
-Qed.
+Time Qed.
