sample_mark/env_binary_heap.v
@@ -1,0 +1,126 @@
+Require Import VST.floyd.proofauto.
+Require Import RamifyCoq.sample_mark.binary_heap.
+Require Import RamifyCoq.sample_mark.binary_heap_model.
+Require Import RamifyCoq.sample_mark.binary_heap_Zmodel.
+Require Import RelationClasses.
+(* Require Import VST.floyd.sublist. *)
+
+Set Nested Proofs Allowed.
+
+(* Relation on heap items. *)
+Definition heap_item : Type := (int * int)%type.
+Definition cmp (a b : heap_item) : bool :=
+  negb (Int.lt (fst b) (fst a)).
+Definition cmp_rel (a b : heap_item) : Prop :=
+  cmp a b = true.
+Lemma cmp_dec: forall a a', {cmp_rel a a'} + {~cmp_rel a a'}.
+Proof.
+  intros [? ?] [? ?]. unfold cmp_rel, cmp. simpl. case (Int.lt i1 i); simpl; auto.
+Qed. 
+Instance cmp_po: PreOrder cmp_rel.
+Proof.
+  constructor. intros [? ?]. red. unfold cmp. simpl. case_eq (Int.lt i i); auto; intro. exfalso.
+  apply lt_inv in H. lia.
+  intros [? ?] [? ?] [? ?]. unfold cmp_rel, cmp. simpl. 
+  case_eq (Int.lt i3 i); auto.
+  case_eq (Int.lt i1 i); auto.
+  case_eq (Int.lt i3 i1); auto. simpl.
+  intros ? ? ?. exfalso.
+  apply lt_inv in H1.
+  apply lt_false_inv in H.
+  apply lt_false_inv in H0.
+  lia.
+Qed.
+Lemma cmp_linear: forall a b,
+  cmp_rel a b \/ cmp_rel b a.
+Proof.
+  intros [? ?] [? ?]. unfold cmp_rel, cmp; simpl.
+  case_eq (Int.lt i1 i); auto. intro. 
+  right.
+  case_eq (Int.lt i i1); auto. intro. exfalso. 
+  apply lt_inv in H. apply lt_inv in H0.
+  lia.
+Qed.
+
+(* Not sure if it's a great idea to expose the capacity inside the abstraction boundary. *)
+Definition heap : Type := (nat * list heap_item)%type.
+Instance heap_inhabitant : Inhabitant heap := (O, []).
+Definition heap_capacity (h : heap) : Z := Z.of_nat (fst h).
+Definition heap_items (h : heap) : list heap_item := snd h.
+Definition heap_size (h : heap) : Z := Zlength (heap_items h).
+
+(*
+Definition heap_permutation (h1 h2 : heap) : Prop :=
+  heap_capacity h1 = heap_capacity h2 /\ Permutation (heap_items h1) (heap_items h2).
+*)
+
+Definition heap_ordered := binary_heap_model.heapOrdered heap_item cmp_rel.
+Definition weak_heap_ordered_bottom_up (L : list heap_item) (x : Z) := 
+  binary_heap_model.weak_heapOrdered2 heap_item cmp_rel L (Z.to_nat x).
+Definition weak_heap_ordered_top_down (L : list heap_item) (x : Z) := 
+  binary_heap_model.weak_heapOrdered heap_item cmp_rel L (Z.to_nat x).
+Definition swim := binary_heap_model.swim heap_item cmp_rel cmp_dec.
+Definition sink L i := binary_heap_model.sink heap_item cmp_rel cmp_dec (L,i).
+(* Definition insert := binary_heap_model.insert heap_item cmp_rel cmp_dec. *)
+(* Definition remove_min := binary_heap_model.remove_min heap_item cmp_rel cmp_dec. *)
+
+Lemma Zparent_repr: forall i,
+  0 < i <= Int.max_unsigned ->
+  Int.repr (Zparent i) = Int.divu (Int.repr (i - 1)) (Int.repr 2).
+Proof.
+  intros. unfold Int.divu. repeat rewrite Int.unsigned_repr.
+  2,3: rep_lia. rewrite Zparent_unfold. trivial. lia.
+Qed.
+
+(* This may get bundled elsewhere at some point. *)
+Instance CompSpecs : compspecs. Proof. make_compspecs prog. Defined.
+Definition Vprog : varspecs. mk_varspecs prog. Defined.
+Global Existing Instance CompSpecs.
+
+Definition t_item := Tstruct _structItem noattr.
+Definition t_pq := Tstruct _structPQ noattr.
+
+Definition heap_item_rep (i : heap_item) : reptype t_item :=
+  (Vint (fst i), Vint (snd i)).
+
+Definition hitem (i : heap_item) : val -> mpred :=
+  data_at Tsh t_item (heap_item_rep i).
+
+Definition harray (contents : list heap_item) : val -> mpred :=
+  data_at Tsh (tarray t_item (Zlength contents)) (map heap_item_rep contents).
+
+Lemma harray_emp: forall arr,
+  harray [] arr |-- emp.
+Proof.
+  unfold harray. intros. rewrite data_at_isptr. entailer. rewrite data_at_zero_array_eq; auto.
+Qed.
+
+Lemma fold_harray': forall L i arr,
+  i = Zlength L ->
+  data_at Tsh (tarray t_item i) (map heap_item_rep L) arr = harray L arr.
+Proof. intros. rewrite H. reflexivity. Qed.
+
+Lemma fold_harray: forall L arr,
+  data_at Tsh (tarray t_item (Zlength L)) (map heap_item_rep L) arr = harray L arr.
+Proof. reflexivity. Qed.
+
+Lemma harray_split: forall L1 L2 ptr,
+  harray (L1 ++ L2) ptr = 
+  ((harray L1 ptr) * 
+   (harray L2 (field_address0 (tarray t_item (Zlength (L1 ++ L2))) [ArraySubsc (Zlength L1)] ptr)))%logic.
+Proof.
+  intros. unfold harray.
+  rewrite map_app.
+  erewrite split2_data_at_Tarray_app.
+  2: rewrite Zlength_map; reflexivity. 2: rewrite Zlength_app, Zlength_map; lia.
+  rewrite Zlength_app.
+  replace (Zlength L1 + Zlength L2 - Zlength L1) with (Zlength L2) by lia.
+  trivial.
+Qed.
+
+Definition valid_pq (pq : val) (h: heap): mpred :=
+  EX arr : val, EX junk: list heap_item,
+    (!! heap_ordered (heap_items h)) && (!! (Zlength ((heap_items h) ++ junk) = heap_capacity h)) &&
+    (!! (2 * (heap_capacity h - 1) <= Int.max_unsigned)) &&
+    (data_at Tsh t_pq (Vint (Int.repr (heap_capacity h)), (Vint (Int.repr (heap_size h)), arr)) pq *
+       harray ((heap_items h) ++ junk) arr).
